investigations/cava2/Fifo.v
@@ -1,0 +1,113 @@
+(****************************************************************************)
+(* Copyright 2021 The Project Oak Authors                                   *)
+(*                                                                          *)
+(* Licensed under the Apache License, Version 2.0 (the "License")           *)
+(* you may not use this file except in compliance with the License.         *)
+(* You may obtain a copy of the License at                                  *)
+(*                                                                          *)
+(*     http://www.apache.org/licenses/LICENSE-2.0                           *)
+(*                                                                          *)
+(* Unless required by applicable law or agreed to in writing, software      *)
+(* distributed under the License is distributed on an "AS IS" BASIS,        *)
+(* WITHOUT WARRANTIES OR CONDITIONS OF ANY KIND, either express or implied. *)
+(* See the License for the specific language governing permissions and      *)
+(* limitations under the License.                                           *)
+(****************************************************************************)
+
+Require Import Coq.Strings.String.
+Require Import Coq.Strings.HexString.
+Require Import Coq.Lists.List.
+Require Import Coq.NArith.NArith.
+
+Require Import Cava.Types.
+Require Import Cava.Expr.
+Require Import Cava.Primitives.
+
+Import ListNotations.
+Import PrimitiveNotations.
+
+Local Open Scope string_scope.
+Local Open Scope N.
+
+Section Var.
+  Import ExprNotations.
+
+  Context {var : tvar}.
+
+  Definition fifo {T} {fifo_size}: Circuit _ [Bit; T; Bit] (Bit ** T ** Bit) :=
+    let fifo_bits := BitVec (Nat.log2 fifo_size) in
+    {{
+    fun data_valid data out_ready =>
+
+    let/delay '(fifo; current_length) :=
+
+      ( if data_valid then data +>> fifo else fifo
+      , if data_valid && !out_ready then current_length + `K 1`
+        else if !data_valid && out_ready && current_length >= `K 1` then (current_length - `K 1`)
+        else current_length
+      )
+
+      initially (@default (Vec T fifo_size), 0)
+        : denote_type (Vec T fifo_size ** fifo_bits) in
+
+    ( current_length >= `K 0`
+    , `index` fifo (current_length - `K 1`)
+    , (current_length >= `Constant ((N.of_nat fifo_size - 1) : denote_type fifo_bits)` ) )
+  }}.
+
+End Var.
+
+Require Import Cava.Semantics.
+Require Import Cava.Util.List.
+Require Import Cava.Util.Tactics.
+
+Definition no_io_predicate (x: denote_type (Bit**BitVec 32**Bit**Unit))
+  := fst x = false /\ fst (snd (snd x)) = false.
+
+Ltac destruct_input input :=
+  match type of input with
+  | denote_type (Pair _ _) =>
+    let x := fresh input in
+    let y := fresh input in
+    destruct input as [x y];
+    destruct_input x; destruct_input y
+  | denote_type Unit => destruct input
+  | _ => idtac
+  end.
+
+Lemma fifo_no_change :
+  forall sz st input, no_io_predicate input ->
+  st = fst (step (fifo (fifo_size:=sz)) st input).
+Proof.
+  intros.
+  cbn [step fifo absorb_any split_absorbed_denotation combine_absorbed_denotation
+    denote_type binary_semantics unary_semantics K
+    ].
+  destruct_input input.
+  unfold no_io_predicate in H.
+  cbn in H.
+  destruct H.
+  rewrite H, H0.
+  repeat (destruct_pair_let; cbn [fst snd]).
+  reflexivity.
+Qed.
+
+Lemma fifo_no_change' :
+  forall sz st inputs,
+  Forall no_io_predicate inputs ->
+  snd (simulate' (fifo (fifo_size:=sz)) inputs st) = st.
+Proof.
+  intros.
+  induction inputs; [reflexivity|].
+  cbv [simulate'] in *.
+  rewrite fold_left_accumulate'_cons_snd.
+  cbn [List.app].
+
+  apply List.Forall_cons_iff in H.
+  destruct H.
+  apply IHinputs in H0.
+  rewrite <- (fifo_no_change _ _ _ H).
+  rewrite fold_left_accumulate'_snd_acc_invariant with (acc_b:=[]%list).
+  apply H0.
+Qed.
+
